theories/Var.v
@@ -32,5 +32,37 @@ Module Ren.
 
 End Ren.
 
+Module Sub.
+  Class syn_struct (𝒯 : Ctx → Type) : Type :=
+    { var : ∀ {Ψ}, Var Ψ → 𝒯 Ψ;
+      map : ∀ {Ψ1 Ψ2}, Ren.t Ψ1 Ψ2 → 𝒯 Ψ1 → 𝒯 Ψ2
+    }.
+
+  Section Sub.
+    Context `{𝒯 : Ctx → Type}.
+    Context `{𝔐 : syn_struct 𝒯}.
+
+    Definition t (Ψ1 Ψ2 : Ctx) := Var Ψ1 → 𝒯 Ψ2.
+
+    Program Definition ren {Ψ1 Ψ2} (ρ : Ren.t Ψ1 Ψ2) : t Ψ1 Ψ2 :=
+      fun x =>
+        var (ρ x).
+
+    Program Definition cong {Ψ1 Ψ2} (σ : t Ψ1 Ψ2) : t (S Ψ1) (S Ψ2) :=
+      fun x =>
+        match x with
+        | Fin.F1 _ => var Fin.F1
+        | Fin.FS _ y => map Fin.FS (σ y)
+        end.
+
+    Program Definition inst0 {Ψ} (e : 𝒯 Ψ) : t (S Ψ) Ψ :=
+      fun x =>
+        match x with
+        | Fin.F1 _ => e
+        | Fin.FS _ y => @var _ 𝔐 _ y
+        end.
+  End Sub.
+End Sub.
+
 Delimit Scope ren_scope with ren.
 Notation "^ n" := (Ren.weak n) (at level 50) : ren_scope.
