theories/ExternalSyn.v
@@ -227,7 +227,7 @@ Proof.
   T.rewrites.
 Qed.
 
-Theorem interp_tm_var_naturality {Λ Ψ0 Ψ1 Ψ2} (e : ETm.t Λ Ψ0) (γ : Tm.Sub.t Ψ1 Ψ2) ρ κs :
+Theorem interp_tm_var_naturality {Λ Ψ0 Ψ1 Ψ2} (e : ETm.t Λ Ψ0) (γ : Sub.t Ψ1 Ψ2) ρ κs :
   (⟦ e ⟧ κs) ⫽ (γ ∘ ρ) = (⟦ e.[ρ] ⟧ κs) ⫽ γ.
 Proof.
   move: Ψ1 Ψ2 γ ρ κs.
@@ -235,14 +235,14 @@ Proof.
   - move=> *; f_equal.
     * by rewrite_all_hyps.
     * rewrite_all_hyps.
-      by rewrite Tm.Sub.cong_coh.
+      by rewrite Tm.cong_coh.
   - move=> *; f_equal; T.eqcd => ?.
     rewrite IHe.
     by rewrite Ren.cong_id.
   - move=> *; f_equal.
     rewrite -IHe.
     f_equal.
-    by rewrite Tm.Sub.cong_coh.
+    by rewrite Tm.cong_coh.
 Qed.
 
 Theorem interp_tm_var_ren_naturality {Λ Ψ0 Ψ1} (e : ETm.t Λ Ψ0) (ρ : Ren.t Ψ0 Ψ1) κs :
