theories/Sequent.v
@@ -33,7 +33,7 @@ Notation "τ ⊧ A ∼ B" := (atomic_eq_ty τ A%tm B%tm) (at level 10).
 Notation "τ ⊧ A ∋ e1 ∼ e2" := (atomic_eq_mem τ A%tm e1%tm e2%tm) (at level 10).
 Reserved Notation "τ ⊧ Γ ∋⋆ γ1 ∼ γ2" (at level 10).
 
-Program Fixpoint atomic_eq_env {Ψ} τ Γ (γ1 γ2 : Tm.Sub.t Ψ 0) : Ω :=
+Program Fixpoint atomic_eq_env {Ψ} τ Γ (γ1 γ2 : Var.Sub.t Ψ 0) : Ω :=
   match Γ with
   | ⋄%ictx => ⊤
   | (Γ ; A)%ictx =>
